\section{Generalization of \cref{thm:submod_cardin}}
\label{sec:submod_cardin_modify}

\begin{theorem}
    Consider a non-negative, monotone, submodular function $f$ and an integer $k$. Let $S^*$ be the set of size $k$ that maximizes $f$ (i.e.\! the optimal solution). 
    Choose some $\varepsilon \in [0, 1 - \frac{1}{e})$.
    There exists some $\gamma \geq 0$ that $\varepsilon$ depends polynomially on such that if $S$ is the set constructed by iteratively choosing $k$ elements that maximize the marginal gain of the function value 
    to within a factor of $\lrp{1-\gamma}$ at each step, 
    then $\func{f}{S} \geq \lrp{1 - \frac{1}{e} - \varepsilon}\func{f}{S^*}$. 
    \label{thm:submod_cardin_gen}
\end{theorem}

Let $S^{\ast} = \lrc{s_1^{\ast}, \ldots, s_k^{\ast}}$ be the optimal solution and $S = \lrc{s_1, \ldots, s_k}$ the solution constructed by the above greedy algorithm.
Define $S_i^{\ast} = \lrc{s_1^{\ast}, \ldots, s_i^{\ast}}$ and similarly $S_i = \lrc{s_1, \ldots, s_i}$ for $i = 0, \ldots, k$, where $S_0^{\ast} = \emptyset = S_0$. 
We first prove the following two claims. 

\begin{claim}
    \begin{equation*}
        \f{S_{i+1}} - \f{S_i} \geq \frac{1-\gamma}{k} \lrp{\f{S_i \cup S^{\ast}} - \f{S_i}} 
        \quad \quad \textnormal{for each } i = 0, \ldots, k-1.
    \end{equation*}
    \label{claim:submod_ineq}
\end{claim}
\begin{proof} 
    Choose some $0 \leq i \leq k-1$. By definition of the greedy approach,
    \begin{align}
        \nonumber 
        \f{S_{i+1}} - \f{S_i} &\geq \lrp{1-\gamma} \lrp{\max_{s \in U} \lrp{\f{S_i \cup \lrc{s}} - \f{S_i}}}  \\
        \label{eq:submod_maximizer}                            
        &\geq \lrp{1-\gamma} \frac{1}{k} \sum_{j=1}^{k} \lrp{\f{S_i \cup \lrc{s_j^{\ast}}} - \f{S_i}}
    \end{align}
    where the second inequality comes from the fact that since $s$ is a maximizer, an average of the marginal gain from others elements in $U$ 
    (in this case specifically in $S^{\ast}$) must be at most the marginal value $s$ provides. 
    
    By submodularity of $f$, 
    \begin{align*}
        \f{S_i \cup \lrc{s_j^{\ast}}} - \f{S_i} &\geq 
        \f{S_i \cup S_{j-1}^{\ast} \cup  \lrc{s_j^{\ast}}} - \f{S_i \cup S_{j-1}^{\ast}} \\&= 
        \f{S_i \cup  S_j^{\ast}} - \f{S_i \cup S_{j-1}^{\ast}}
    \end{align*}
    since $S_i \sse S_i \cup S_{j-1}^{\ast}$. Using this inequality with \cref{eq:submod_maximizer}, we get
    \begin{align*}
        \f{S_{i+1}} - \f{S_i} &\geq \frac{1-\gamma}{k} \sum_{j=1}^{k} \lrp{\f{S_i \cup  S_j^{\ast}} - \f{S_i \cup S_{j-1}^{\ast}}}\\
        &= \frac{1-\gamma}{k} \lrp{\f{S_i \cup S_k^{\ast}} - \f{S_i \cup S_0^{\ast}}}\\
        &= \frac{1-\gamma}{k} \lrp{\f{S_i \cup S^{\ast}} - \f{S_i}}
    \end{align*}
    where the equality comes from the fact that the summation telescopes. 
\end{proof}

\begin{claim}
    \begin{equation*}
        \f{S_i} \geq \lrp{1 - \lrp{1 - \frac{1}{k}}^i - \varepsilon}\f{S^{\ast}} \quad \quad 
        \textnormal{for each } i = 1, \ldots, k 
    \end{equation*}
    where $\varepsilon$ is equivalent to some polynomial function of $\gamma$. 
    \label{claim:submod_ineq_induction}
\end{claim}
\begin{proof}
    To simplify analysis, we assume WLOG that $\f{\emptyset} = 0$. We prove by induction. 
    The base case follows from \cref{claim:submod_ineq}:
    \begin{align*}
        \f{S_1} = \f{S_1} - \f{S_0} &\geq \frac{1 - \gamma}{k} \lrp{\f{S_0 \cup  S^{\ast}} - \f{S_0}} \\
        &> \lrp{\frac{1}{k} - \gamma} \f{S^{\ast}}
        %&> \lrp{1 - \lrp{1 - \frac{1}{k}} - \frac{\gamma k^2 + \gamma - \gamma^2 k}{k^2}} \f{S^{\ast}}
    \end{align*}
    %where $\varepsilon = \frac{\gamma k^2 + \gamma - \gamma^2 k}{k^2}$. For the induction case, assume the claim holds for $i = j$. Then, 
    where $\varepsilon = \gamma$. For the induction case, assume the claim holds for $i = j$. Then, 
    \begin{align*}
        \f{S_{j+1}} - \f{S_j} &\geq \frac{1-\gamma}{k} \lrp{\f{S_j \cup  S^{\ast}} - \f{S_j}}
        \tag*{(by \cref{claim:submod_ineq})}\\
        &\geq \frac{1-\gamma}{k} \lrp{\f{S^{\ast}} - \f{S_j}}\\
        \f{S_{j+1}} &\geq \frac{1-\gamma}{k} \f{S^{\ast}} + \frac{k - 1 + \gamma}{k} \f{S_j}\\
        &\geq \frac{1-\gamma}{k} \f{S^{\ast}} + \frac{k-1+\gamma}{k}\lrp{1 - \lrp{1 - \frac{1}{k}}^j - \gamma} \f{S^{\ast}}
        \tag*{(by ind. hyp.)}\\ 
        &= \f{S^{\ast}} \lrp{\frac{1}{k} - \frac{\gamma}{k} + \lrp{1 - \frac{1}{k} + \frac{\gamma}{k}} \lrp{1 - \lrp{1 - \frac{1}{k}} - \gamma}} \\
        &= \f{S^{\ast}} \lrp{1 - \lrp{1 - \frac{1}{k}}^{j+1} -\gamma + \frac{\gamma}{k} \lrp{1 - \lrp{1 - \frac{1}{k}}^j - \gamma}} 
        \\
        &\geq \f{S^{\ast}} \lrp{1 - \lrp{1 - \frac{1}{k}}^{j+1} -\gamma + \frac{\gamma}{k} \lrp{\frac{1}{k} - \gamma}} 
        \tag*{($j = 1$ is the maximizer)}\\
        &= \f{S^{\ast}} \lrp{1 - \lrp{1 - \frac{1}{k}}^{j+1} - \lrp{\frac{\gamma k^2 - \gamma + \gamma^2 k}{k^2}}}
    \end{align*} 
    where $\varepsilon = \frac{\gamma k^2 - \gamma + \gamma^2 k}{k^2}$, which proves the induction case. 
\end{proof}

%Using the previous claim gives the proof of \cref{thm:submod_cardin_gen} as an immediate consequence. 
\begin{proof}[of \cref{thm:submod_cardin_gen}]
    Take $i = k$ in \cref{claim:submod_ineq_induction}. Then 
    \begin{equation*}
        \f{S_k} = \f{S} \geq \lrp{1 - \lrp{1 - \frac{1}{k}}^k - \varepsilon}\f{S^{\ast}} > \lrp{1 - \frac{1}{e} - \varepsilon}\f{S^{\ast}}. 
    \end{equation*}
    To find the appropriate $\gamma$ value, solve the quadratic equation $\gamma^2k + \gamma \lrp{k^2-1} - \varepsilon k^2 = 0$ and take the non-negative root.  
\end{proof}
